Change eval rules such that Axiom equating FMap Equal to Logic.eq is no longer needed for the soundness proof

proof_of_soundness/EvalRules.v
@@ -91,20 +91,23 @@ Inductive EvalExpr:
   Z -> store -> Prop :=
   (* Numerals evaluate to their integer representation and do not
      change the store *)
-  | E_Num : forall S E G F M z,
-    EvalExpr S E G F M (Num z) z S
+  | E_Num : forall S E G F M z S',
+    NatMap.Equal S S' ->
+    EvalExpr S E G F M (Num z) z S'
   (* Variable lookup occurs iff a macro parameter is not found. *)
-  | E_LocalVar : forall S E G F M x l v,
+  | E_LocalVar : forall S E G F M x l v S',
+    NatMap.Equal S S' ->
     StringMap.MapsTo x l E ->
     NatMap.MapsTo l v S ->
-    EvalExpr S E G F M (Var x) v S
+    EvalExpr S E G F M (Var x) v S'
   (* Local variables shadow global variables, so only if a local
      variable lookup fails do we check the global environment. *)
-  | E_GlobalVar : forall S E G F M x l v,
+  | E_GlobalVar : forall S E G F M x l v S',
+    NatMap.Equal S S' ->
     ~ StringMap.In x E->
     StringMap.MapsTo x l G ->
     NatMap.MapsTo l v S ->
-    EvalExpr S E G F M (Var x) v S
+    EvalExpr S E G F M (Var x) v S'
   (* Parenthesized expressions evaluate to themselves. *)
   | E_ParenExpr : forall S E G F M e0 v S',
     EvalExpr S E G F M e0 v S' ->
@@ -131,14 +134,14 @@ Inductive EvalExpr:
   | E_Assign_Local : forall S E G F M l x e0 v S' S'',
     StringMap.MapsTo x l E ->
     EvalExpr S E G F M e0 v S' ->
-    S'' = NatMapProperties.update S (NatMap.add l v (NatMap.empty Z)) ->
+    NatMap.Equal S'' (NatMapProperties.update S (NatMap.add l v (NatMap.empty Z))) ->
     EvalExpr S E G F M (Assign x e0) v S''
   (* Global variable assignment *)
   | E_Assign_Global : forall S E G F M l x e0 v S' S'',
     ~ StringMap.In x E ->
     StringMap.MapsTo x l G ->
     EvalExpr S E G F M e0 v S' ->
-    S'' = NatMapProperties.update S (NatMap.add l v (NatMap.empty Z)) ->
+    NatMap.Equal S'' (NatMapProperties.update S (NatMap.add l v (NatMap.empty Z))) ->
     EvalExpr S E G F M (Assign x e0) v S''
   (* For function calls, we perform the following steps:
      1) Evaluate arguments
@@ -173,7 +176,7 @@ Inductive EvalExpr:
        We could possibly prove this, but it is easier to put it here. *)
     NatMapProperties.Disjoint S' Sargs ->
     (* Combine the argument store into the original store *)
-    S'' = NatMapProperties.update S' Sargs ->
+    NatMap.Equal S'' (NatMapProperties.update S' Sargs) ->
     (* Evaluate the function's body *)
     EvalStmt S'' Ef G F M fstmt S''' ->
     EvalExpr S''' Ef G F M fexpr v S'''' ->
@@ -204,11 +207,12 @@ with EvalExprList :
   list string -> list expr -> list Z -> store -> environment -> store ->
   nat -> list nat -> Prop :=
   (* End of arguments *)
-  | EvalExprList_nil : forall Sprev Ecaller G F M,
-    EvalExprList Sprev Ecaller G F M nil nil nil Sprev (StringMap.empty nat) (NatMap.empty Z)
+  | E_ExprList_nil : forall Sprev Ecaller G F M Snext,
+    NatMap.Equal Sprev Snext ->
+    EvalExprList Sprev Ecaller G F M nil nil nil Snext (StringMap.empty nat) (NatMap.empty Z)
       1 (0 :: nil)
   (* There are arguments left to evaluate *)
-  | EvalExprList_cons : forall Sprev Ecaller G F M p e v Snext ps es vs Sfinal Ef' Sargs' l ls,
+  | E_ExprList_cons : forall Sprev Ecaller G F M p e v Snext ps es vs Sfinal Ef' Sargs' l ls,
     (* Evaluate the first expression using the caller's environment *)
     EvalExpr Sprev Ecaller G F M e v Snext ->
     (* Evaluate the remaining expressions *)
@@ -235,8 +239,9 @@ with EvalStmt :
   stmt ->
   store -> Prop :=
   (* A skip statement does not change the state *)
-  | E_Skip : forall S E G F M,
-    EvalStmt S E G F M Skip S.
+  | E_Skip : forall S E G F M S',
+    NatMap.Equal S S' ->
+    EvalStmt S E G F M Skip S'.
 
 
 Scheme MSub_mut := Induction for MSub Sort Prop
@@ -337,7 +342,8 @@ Lemma EvalStmt_Disjoint_update_F_EvalStmt : forall S E G F M stmt S',
     StringMapProperties.Disjoint F F' ->
     EvalStmt S E G (StringMapProperties.update F F') M stmt S'.
 Proof.
-  intros. induction H; try constructor. Qed.
+  intros. induction H; try constructor. auto.
+Qed.
 
 
 Lemma EvalExpr_notin_F_add_EvalExpr : forall S E G F M e v S',
@@ -376,7 +382,7 @@ Proof.
         contradiction.
       * auto.
   - apply E_MacroInvocation with params mexpr M' ef; auto.
-  - apply EvalExprList_cons with Snext; auto.
+  - apply E_ExprList_cons with Snext; auto.
 Qed.
 
 
@@ -422,7 +428,7 @@ Proof.
         -- contradiction.
         -- auto.
   - apply E_MacroInvocation with params mexpr M' ef; auto.
-  - apply EvalExprList_cons with Snext; auto.
+  - apply E_ExprList_cons with Snext; auto.
 Qed.
 
 
@@ -468,7 +474,7 @@ Proof.
         -- contradiction.
         -- auto.
   - apply E_MacroInvocation with params mexpr M' ef; auto.
-  - apply EvalExprList_cons with Snext; auto.
+  - apply E_ExprList_cons with Snext; auto.
 Qed.
 
 
@@ -507,7 +513,7 @@ Proof.
         contradiction.
       * auto.
   - apply E_MacroInvocation with params mexpr M' ef; auto.
-  - apply EvalExprList_cons with Snext; auto.
+  - apply E_ExprList_cons with Snext; auto.
 Qed.
 
 
@@ -553,7 +559,7 @@ Proof.
         -- contradiction.
         -- auto.
   - apply E_MacroInvocation with params mexpr M' ef; auto.
-  - apply EvalExprList_cons with Snext; auto.
+  - apply E_ExprList_cons with Snext; auto.
 Qed.
 
 
@@ -562,8 +568,216 @@ Lemma EvalExpr_Var_x_in_E_or_G : forall S E G F M x v S',
   StringMap.In x E \/ StringMap.In x G.
 Proof.
   intros. inversion_clear H.
-  - left. apply StringMap_mapsto_in in H0. auto.
-  - right. apply StringMap_mapsto_in in H1. auto.
+  - left. apply StringMap_mapsto_in in H1. auto.
+  - right. apply StringMap_mapsto_in in H2. auto.
+Qed.
+
+
+Lemma S_Equal_EvalExpr : forall S_1 E G F M e v S',
+  EvalExpr S_1 E G F M e v S' ->
+  forall S_2,
+  NatMap.Equal S_1 S_2 ->
+  EvalExpr S_2 E G F M e v S'.
+Proof.
+  apply (EvalExpr_mut
+      (* EvalExpr *)
+      (fun S_1 E G F M e v S' (h : EvalExpr S_1 E G F M e v S' ) =>
+        forall S_2,
+        NatMap.Equal S_1 S_2 ->
+        EvalExpr S_2 E G F M e v S')
+      (* EvalStmt *)
+      (fun S_1 E G F M stmt S' (h : EvalStmt S_1 E G F M stmt S' ) =>
+        forall S_2,
+        NatMap.Equal S_1 S_2 ->
+        EvalStmt S_2 E G F M stmt S')
+      (* EvalExprList *)
+      (fun S_1 Ecaller G F M ps es vs Snext Ef Sargs l ls
+        (h : EvalExprList S_1 Ecaller G F M ps es vs Snext Ef Sargs l ls) =>
+        forall S_2,
+        NatMap.Equal S_1 S_2 ->
+        EvalExprList S_2 Ecaller G F M ps es vs Snext Ef Sargs l ls)
+    ); intros.
+  - (* Num *)
+    rewrite H in e. constructor; auto.
+  - (* Local var *)
+    rewrite H in e. apply E_LocalVar with l; auto. rewrite <- H; auto.
+  - (* Global var *)
+     rewrite H in e; apply E_GlobalVar with l; auto. rewrite <- H; auto.
+  - (* ParenExpr *)
+     constructor. apply H; auto.
+  - (* UnExpr *)
+     constructor. apply H; auto.
+  - (* BinExpr *)
+      apply E_BinExpr with S'.
+      * (* Left operand *)
+        apply H. auto.
+      * (* Right operand *)
+        apply H0; reflexivity.
+  - (* Local assignment *)
+    rewrite H0 in e1. apply E_Assign_Local with l S'; auto.
+  - (* Global assignment *)
+    rewrite H0 in e1. apply E_Assign_Global with l S'; auto.
+  - (* Function call *)
+    rewrite H2 in e5.
+    apply E_FunctionCall with params fstmt fexpr l ls Ef Sargs S' S'' S''' S'''' vs; auto.
+  - (* Macro invocation *)
+    apply E_MacroInvocation with params mexpr M' ef; auto.
+  - (* Statements *)
+    constructor. rewrite H in e; auto.
+  - (* ExprList (nil) *)
+    constructor. rewrite H in e; auto.
+  - (* ExprList (cons) *)
+    apply E_ExprList_cons with Snext; auto.
+Qed.
+
+
+Lemma S'_Equal_EvalExpr : forall S E G F M e v S'_1,
+  EvalExpr S E G F M e v S'_1 ->
+  forall S'_2,
+  NatMap.Equal S'_1 S'_2 ->
+  EvalExpr S E G F M e v S'_2.
+Proof.
+  apply (EvalExpr_mut
+      (* EvalExpr *)
+      (fun S E G F M e v S'_1 (h : EvalExpr S E G F M e v S'_1 ) =>
+        forall S'_2,
+        NatMap.Equal S'_1 S'_2 ->
+        EvalExpr S E G F M e v S'_2)
+      (* EvalStmt *)
+      (fun S E G F M stmt S'_1 (h : EvalStmt S E G F M stmt S'_1 ) =>
+        forall S'_2,
+        NatMap.Equal S'_1 S'_2 ->
+        EvalStmt S E G F M stmt S'_2)
+      (* EvalExprList *)
+      (fun S Ecaller G F M ps es vs Snext_1 Ef Sargs l ls
+        (h : EvalExprList S Ecaller G F M ps es vs Snext_1 Ef Sargs l ls) =>
+        forall Snext_2,
+        NatMap.Equal Snext_1 Snext_2 ->
+        EvalExprList S Ecaller G F M ps es vs Snext_2 Ef Sargs l ls)
+    ); intros.
+  - (* Num *)
+    rewrite H in e. constructor; auto.
+  - (* Local var *)
+    rewrite H in e. apply E_LocalVar with l; auto.
+  - (* Global var *)
+     rewrite H in e; apply E_GlobalVar with l; auto.
+  - (* ParenExpr *)
+     constructor. apply H; auto.
+  - (* UnExpr *)
+     constructor. apply H; auto.
+  - (* BinExpr *)
+      apply E_BinExpr with S'.
+      * (* Left operand *)
+        apply H. reflexivity.
+      * (* Right operand *)
+        apply H0. auto.
+  - (* Local assignment *)
+    rewrite H0 in e1. apply E_Assign_Local with l S'; auto.
+  - (* Global assignment *)
+    rewrite H0 in e1. apply E_Assign_Global with l S'; auto.
+  - (* Function call *)
+    rewrite H2 in e5.
+    apply E_FunctionCall with params fstmt fexpr l ls Ef Sargs S' S'' S''' S'''' vs; auto.
+  - (* Macro invocation *)
+    apply E_MacroInvocation with params mexpr M' ef; auto.
+  - (* Statements *)
+    constructor. rewrite H in e; auto.
+  - (* ExprList (nil) *)
+    constructor. rewrite H in e; auto.
+  - (* ExprList (cons) *)
+    apply E_ExprList_cons with Snext; auto.
+Qed.
+
+
+Lemma S_Equal_EvalExprList : forall S_1 Ecaller G F M ps es vs Snext Ef Sargs l ls,
+  EvalExprList S_1 Ecaller G F M ps es vs Snext Ef Sargs l ls ->
+  forall S_2,
+  NatMap.Equal S_1 S_2 ->
+  EvalExprList S_2 Ecaller G F M ps es vs Snext Ef Sargs l ls.
+Proof.
+  intros S_1 Ecaller G F M ps es vs Snext Ef Sargs l ls H. induction H; intros.
+  - (* ExprList nil *)
+    constructor. rewrite H0 in H. auto.
+  - (* ExprList cons *)
+    apply E_ExprList_cons with Snext; auto.
+    eapply S_Equal_EvalExpr; eauto.
+Qed.
+
+
+Lemma S_Equal_EvalStmt : forall S_1 E G F M st S',
+  EvalStmt S_1 E G F M st S' ->
+  forall S_2,
+  NatMap.Equal S_1 S_2 ->
+  EvalStmt S_2 E G F M st S'.
+Proof.
+  intros S_1 E G F M st S' H. induction H; intros.
+  - (* Skip *)
+    constructor. rewrite H0 in H. auto.
+Qed.
+
+
+Lemma E_Equal_EvalExpr : forall S E_1 G F M e v S',
+  EvalExpr S E_1 G F M e v S' ->
+  forall E_2,
+  StringMap.Equal E_1 E_2 ->
+  EvalExpr S E_2 G F M e v S'.
+Proof.
+  apply (EvalExpr_mut
+      (* EvalExpr *)
+      (fun S E_1 G F M e v S' (h : EvalExpr S E_1 G F M e v S' ) =>
+        forall E_2,
+        StringMap.Equal E_1 E_2 ->
+        EvalExpr S E_2 G F M e v S')
+      (* EvalStmt *)
+      (fun S E_1 G F M stmt S' (h : EvalStmt S E_1 G F M stmt S' ) =>
+        forall E_2,
+        StringMap.Equal E_1 E_2 ->
+        EvalStmt S E_2 G F M stmt S')
+      (* EvalExprList *)
+      (fun S Ecaller_1 G F M ps es vs Snext Ef Sargs l ls
+        (h : EvalExprList S Ecaller_1 G F M ps es vs Snext Ef Sargs l ls) =>
+        forall Ecaller_2,
+        StringMap.Equal Ecaller_1 Ecaller_2 ->
+        EvalExprList S Ecaller_2 G F M ps es vs Snext Ef Sargs l ls)
+    ); intros.
+  - (* Num *)
+    constructor; auto.
+  - (* Local var *)
+    apply E_LocalVar with l; auto. rewrite H in m. auto.
+  - (* Global var *)
+    apply E_GlobalVar with l; auto. rewrite H in n. auto.
+  - (* ParenExpr *)
+    constructor; auto.
+  - (* UnExpr *)
+    constructor; auto.
+  - (* BinExpr *)
+    apply E_BinExpr with S'; auto.
+  - (* Local assignment *)
+    apply E_Assign_Local with l S'; auto. rewrite H0 in m. auto.
+  - (* Global assignment *)
+    apply E_Assign_Global with l S'; auto. rewrite H0 in n. auto.
+  - (* Function call *)
+    apply E_FunctionCall with params fstmt fexpr l ls Ef Sargs S' S'' S''' S'''' vs; auto.
+  - (* Macro invocation *)
+    apply E_MacroInvocation with params mexpr M' ef; auto.
+  - (* Statements *)
+    constructor; auto.
+  - (* ExprList (nil) *)
+    constructor; auto.
+  - (* ExprList (cons) *)
+    apply E_ExprList_cons with Snext; auto.
+Qed.
+
+
+Lemma E_Equal_EvalStmt : forall S E_1 G F M st S',
+  EvalStmt S E_1 G F M st S' ->
+  forall E_2,
+  StringMap.Equal E_1 E_2 ->
+  EvalStmt S E_2 G F M st S'.
+Proof.
+  intros S_1 E G F M st S' H. induction H; intros.
+  - (* Skip *)
+    constructor; auto.
 Qed.
 
 
@@ -571,142 +785,133 @@ Lemma EvalExpr_deterministic : forall S E G F M e v1 S'1,
   EvalExpr S E G F M e v1 S'1 ->
   forall v2 S'2,
   EvalExpr S E G F M e v2 S'2 ->
-  v1 = v2 /\ S'1 = S'2.
+  v1 = v2 /\ NatMap.Equal S'1 S'2.
 Proof.
   apply (EvalExpr_mut
       (* EvalExpr *)
       (fun S E G F M e v1 S'1 (h : EvalExpr S E G F M e v1 S'1 ) =>
         forall v2 S'2,
           EvalExpr S E G F M e v2 S'2 ->
-          v1 = v2 /\ S'1 = S'2)
+          v1 = v2 /\ NatMap.Equal S'1 S'2)
       (* EvalStmt *)
       (fun S E G F M stmt S'1 (h : EvalStmt S E G F M stmt S'1 ) =>
         forall S'2,
           EvalStmt S E G F M stmt S'2 ->
-          S'1 = S'2)
+          NatMap.Equal S'1 S'2)
       (* EvalExprList *)
       (fun Sprev Ecaller G F M ps es vs1 Snext1 Ef1 Sargs1 l1 ls1
         (h : EvalExprList Sprev Ecaller G F M ps es vs1 Snext1 Ef1 Sargs1 l1 ls1) =>
         forall vs2 Snext2 Ef2 Sargs2 l2 ls2,
           EvalExprList Sprev Ecaller G F M ps es vs2 Snext2 Ef2 Sargs2 l2 ls2 ->
-          vs1 = vs2 /\ Snext1 = Snext2 /\ Ef1 = Ef2 /\ Sargs1 = Sargs2 /\ l1 = l2 /\ ls1 = ls2)
+          vs1 = vs2 /\ NatMap.Equal Snext1 Snext2 /\ StringMap.Equal Ef1 Ef2 /\ NatMap.Equal Sargs1 Sargs2 /\ l1 = l2 /\ ls1 = ls2)
     ); intros; auto.
-
   - (* Num *)
-    inversion_clear H. auto.
-
+    inversion_clear H. split; auto.
+    rewrite H0 in e. symmetry in e. auto.
   - (* Local Var *)
-    assert (S = S'2).
-    { inversion_clear H; auto. }
-    subst S'2.
     inversion_clear H.
     + (* Local *)
       assert (l=l0). { eapply StringMapFacts.MapsTo_fun; eauto. }
       subst l0.
       assert (v=v2). { eapply NatMapFacts.MapsTo_fun; eauto. }
-      subst v2; auto.
+      subst v2; split; auto. rewrite <- e. auto.
     + (* Global (contradiction *)
       apply StringMap_mapsto_in in m. contradiction.
-
   - (* Global Var *)
-    assert (S = S'2).
-    { inversion_clear H; auto. }
-    subst S'2.
     inversion_clear H.
     + (* Local *)
-      apply StringMap_mapsto_in in H0. contradiction.
+      apply StringMap_mapsto_in in H1. contradiction.
     + (* Global (contradiction *)
       assert (l=l0). { eapply StringMapFacts.MapsTo_fun; eauto. }
       subst l0.
       assert (v=v2). { eapply NatMapFacts.MapsTo_fun; eauto. }
-      subst v2; auto.
-
+      subst v2; split; auto. rewrite <- H0. symmetry. auto.
   - (* ParenExpr *)
-    inversion_clear H0. auto.
-
-- (* UnExpr *)
+    inversion_clear H0; auto.
+  - (* UnExpr *)
+      inversion_clear H0.
+      destruct H with v0 S'2; auto. subst. auto.
+  - (* BinExpr *)
+    inversion_clear H1.
+    (* Left operand*)
+    assert (v1 = v3 /\ NatMap.Equal S' S'0). { auto. }
+    destruct H1; subst.
+    (* Right operand *)
+    assert (v2 = v4 /\ NatMap.Equal S'' S'2).
+    { apply H0. apply S_Equal_EvalExpr with S'0; auto. symmetry. auto. }
+    destruct H1; subst.
+    auto.
+  - (* Local Assignment *)
     inversion_clear H0.
-    destruct H with v0 S'2; auto. subst. auto.
+    + (* Local assignment *)
+      assert (v = v2 /\ NatMap.Equal S' S'0). { auto. }
+      destruct H0. subst v2.
+      assert (l0 = l). { eapply StringMapFacts.MapsTo_fun; eauto. }
+      subst. rewrite <- H3 in e1. auto.
+    + (* Global assignment (contradiction) *)
+      apply StringMap_mapsto_in in m. contradiction.
+  - (* Global Assignment *)
+    inversion_clear H0.
+    + (* Local assignment (contradiction) *)
+      apply StringMap_mapsto_in in H1. contradiction.
+    + (* Global assignment *)
+      assert (v = v2 /\ NatMap.Equal S' S'0). { auto. }
+      destruct H0. subst v2.
+      assert (l0 = l). { eapply StringMapFacts.MapsTo_fun; eauto. }
+      subst. auto. rewrite <- H4 in e1. auto.
+  - (* Function call *)
+    inversion_clear H2.
+    + (* Function call *)
+      assert ((params0, fstmt0, fexpr0) = (params, fstmt, fexpr)).
+      { eapply StringMapFacts.MapsTo_fun; eauto. }
+      inversion H2; subst params0 fstmt0 fexpr0; clear H2.
+      assert (vs = vs0 /\ NatMap.Equal S' S'0 /\ StringMap.Equal Ef Ef0 /\ NatMap.Equal Sargs Sargs0 /\ l = l0 /\ ls = ls0). { auto. }
+      destruct H2. destruct H14. destruct H15. destruct H16. destruct H17. subst vs0 l0 ls0.
+      assert (NatMap.Equal S'' S''0).
+      { rewrite <- H14 in H10. rewrite <- H16 in H10. rewrite <- e2 in H10. symmetry. auto. }
+      assert (NatMap.Equal S''' S'''0). symmetry in H2. symmetry in H15.
+      { apply S_Equal_EvalStmt with (S_2:=S'') in H11; auto.
+        apply E_Equal_EvalStmt with (E_2:=Ef) in H11; auto. }
+      assert (v = v2 /\ NatMap.Equal S'''' S''''0).
+      symmetry in H17. symmetry in H15.
+      { apply S_Equal_EvalExpr with (S_2:=S''') in H12; auto. 
+        apply E_Equal_EvalExpr with (E_2:=Ef) in H12; auto. }
+      destruct H18. subst v2. rewrite H19 in e5.
+      rewrite <- e5 in H13. symmetry in H13. auto.
+    + (* Macro invocation (contradiction) *)
+      apply StringMap_mapsto_in in H3. contradiction.
+  - (* Macro invocation *)
+    inversion_clear H0.
+    + (* Function call (contradiction) *)
+      apply StringMap_mapsto_in in m. contradiction.
+    + (* Macro invocation *)
+      assert ((params0, mexpr0) = (params, mexpr)).
+      { eapply StringMapFacts.MapsTo_fun; eauto. }
+      inversion H0. subst params0 mexpr0. clear H0.
+      assert (ef = ef0).
+      { eapply MacroSubst_deterministic; eauto. }
+      subst ef0.
+      assert (M' = M'0). { subst. auto. }
+      rewrite <- H0 in *.
+      apply H; auto.
+  - (* Statements *)
+    inversion_clear H. rewrite e in H0. auto.
+  - (* EvalExprList nil *)
+    inversion_clear H. rewrite e in H0. repeat (split; auto; try reflexivity).
 
-- (* BinExpr *)
-  inversion_clear H1.
-
-  (* Left operand*)
-  assert (v1 = v3 /\ S' = S'0). { auto. }
-  destruct H1; subst.
-
-  (* Right operand *)
-  assert (v2 = v4 /\ S'' = S'2). { auto. }
-  destruct H1; subst.
-  auto.
-
-- (* Local Assignment *)
-  inversion_clear H0.
-  + (* Local assignment *)
-    assert (v = v2 /\ S' = S'0). { auto. }
-    destruct H0. subst v2 S'0.
-    assert (l0 = l). { eapply StringMapFacts.MapsTo_fun; eauto. }
-    subst. auto.
-  + (* Global assignment (contradiction) *)
-    apply StringMap_mapsto_in in m. contradiction.
-
-- (* Global Assignment *)
-  inversion_clear H0.
-  + (* Local assignment (contradiction) *)
-    apply StringMap_mapsto_in in H1. contradiction.
-
-  + (* Global assignment *)
-    assert (v = v2 /\ S' = S'0). { auto. }
-    destruct H0. subst v2 S'0.
-    assert (l0 = l). { eapply StringMapFacts.MapsTo_fun; eauto. }
-    subst. auto.
-
-- (* Function call *)
-  inversion_clear H2.
-  + (* Function call *)
-    assert ((params0, fstmt0, fexpr0) = (params, fstmt, fexpr)).
-    { eapply StringMapFacts.MapsTo_fun; eauto. }
-    inversion H2; subst params0 fstmt0 fexpr0; clear H2.
-    assert (vs = vs0 /\ S' = S'0 /\ Ef = Ef0 /\ Sargs = Sargs0 /\ l = l0 /\ ls = ls0). { auto. }
-    destruct H2. destruct H14. destruct H15. destruct H16. destruct H17. subst vs0 S'0 Ef0 Sargs0 l0 ls0.
-   assert (S'' = S''0). { subst; auto. }
-   rewrite <- H2 in *. clear H2. assert (S''' = S'''0). { auto. }
-   subst S'''0. assert (v = v2 /\ S'''' = S''''0). { auto. }
-   destruct H2. subst v2 S''''0.
-   rewrite <- e5 in H13. apply NatMap_Equal_eq_iff in H13. subst. auto.
-  + (* Macro invocation (contradiction) *)
-    apply StringMap_mapsto_in in H3. contradiction.
-
-- (* Macro invocation *)
-  inversion_clear H0.
-  + (* Function call (contradiction) *)
-    apply StringMap_mapsto_in in m. contradiction.
-  + (* Macro invocation *)
-    assert ((params0, mexpr0) = (params, mexpr)).
-    { eapply StringMapFacts.MapsTo_fun; eauto. }
-    inversion H0. subst params0 mexpr0. clear H0.
-    assert (ef = ef0).
-    { eapply MacroSubst_deterministic; eauto. }
-    subst ef0.
-    assert (M' = M'0). { subst. auto. }
-    rewrite <- H0 in *.
-    apply H; auto.
-
-- (* Stmt *)
-  inversion_clear H. auto.
-
-- (* EvalExprList nil *)
-  inversion_clear H. split; auto.
-
-- (* EvalExprList cons *)
-  inversion_clear H1.
-  assert (v = v0 /\ Snext = Snext0). { auto. }
-  destruct H1. subst v0 Snext0.
-  assert (vs = vs0 /\ Sfinal = Snext2 /\ Ef' = Ef'0 /\ Sargs' = Sargs'0 /\ l = l2 /\ ls = ls0).
-  { auto. }
-  destruct H1. destruct H7. destruct H8. destruct H9. destruct H10. subst.
-  split; auto.
+  - (* EvalExprList cons *)
+    inversion_clear H1.
+    assert (v = v0 /\ NatMap.Equal Snext Snext0). { auto. }
+    destruct H1. subst v0.
+    assert (vs = vs0 /\ NatMap.Equal Sfinal Snext2 /\ StringMap.Equal Ef' Ef'0 /\ NatMap.Equal Sargs' Sargs'0 /\ l = l2 /\ ls = ls0).
+    { symmetry in H7. apply S_Equal_EvalExprList with (S_2:=Snext) in H3; auto. }
+    destruct H1. destruct H8. destruct H9. destruct H10. destruct H11. subst.
+    split; auto. split; auto.
+    split. rewrite H9. reflexivity.
+    split. rewrite H10. reflexivity.
+    auto.
 Qed.
+
 
 
 
